% This file was converted to LaTeX by Writer2LaTeX ver. 1.1.3
% see http://writer2latex.sourceforge.net for more info
\documentclass[letterpaper]{article}
\usepackage[latin1]{inputenc}
\usepackage[T1]{fontenc}
\usepackage[english]{babel}
\usepackage{amsmath}
\usepackage{amssymb,amsfonts,textcomp}
\usepackage{color}
\usepackage{array}
\usepackage{supertabular}
\usepackage{hhline}
\usepackage{hyperref}
\hypersetup{pdftex, colorlinks=true, linkcolor=blue, citecolor=blue, filecolor=blue, urlcolor=blue, pdftitle=, pdfauthor=James Brooks, pdfsubject=, pdfkeywords=}
% Outline numbering
\setcounter{secnumdepth}{0}
\makeatletter
\newcommand\arraybslash{\let\\\@arraycr}
\makeatother
% Page layout (geometry)
\setlength\voffset{-1in}
\setlength\hoffset{-1in}
\setlength\topmargin{2cm}
\setlength\oddsidemargin{2cm}
\setlength\textheight{23.94cm}
\setlength\textwidth{17.59cm}
\setlength\footskip{0.0cm}
\setlength\headheight{0cm}
\setlength\headsep{0cm}
% Footnote rule
\setlength{\skip\footins}{0.119cm}
\renewcommand\footnoterule{\vspace*{-0.018cm}\setlength\leftskip{0pt}\setlength\rightskip{0pt plus 1fil}\noindent\textcolor{black}{\rule{0.25\columnwidth}{0.018cm}}\vspace*{0.101cm}}
% Pages styles
\makeatletter
\newcommand\ps@Standard{
  \renewcommand\@oddhead{}
  \renewcommand\@evenhead{}
  \renewcommand\@oddfoot{}
  \renewcommand\@evenfoot{}
  \renewcommand\thepage{\arabic{page}}
}
\makeatother
\pagestyle{Standard}
\setlength\tabcolsep{1mm}
\renewcommand\arraystretch{1.3}
\title{}
\author{James Brooks}
\date{2008-02-18}
\begin{document}
\section{Machine Equations }
James Brooks - Monday 21 May 2007

Taken from - [Chan 92 p.12]

\begin{equation*}
\begin{gathered}I_{d}=Y_{\Re
}(E_{d}''-V_{d})-Y_{d}''(E_{q}''-V_{q})\\I_{q}=Y_{\Re
}(E_{q}''-V_{q})+Y_{q}''(E_{d}''-V_{d})\\\mathit{pE}_{d}''=\frac{1}{T_{\mathit{qo}''}}\{(x_{q}-x_{q}'')I_{q}-E_{d}''-\mathit{aE}_{d}''\}\\\mathit{pE}_{q}'=\frac{1}{T_{\mathit{do}'}}\{V_{f}-(x_{d}-x_{d}')I_{d}-E_{q}'-\mathit{aE}_{q}'\}\\\mathit{pE}_{q}''=\frac{1}{T_{\mathit{do}''}}\{E_{q}'+\mathit{aE}_{q}'-(x_{d}'-x_{d}'')I_{d}-E_{q}''-\mathit{aE}_{q}''\}\end{gathered}
\end{equation*}
Where:

\begin{equation*}
Y_{d}''=-{\frac{X_{q}''}{(R_{a})^{2}+(X_{d}''\times X_{q}'')}}
\end{equation*}
\begin{equation*}
Y_{q}=-{\frac{X_{d}''}{(R_{a})^{2}+(X_{d}''\times X_{q}'')}}
\end{equation*}
\begin{equation*}
Y_{\Re }=\frac{R_{a}}{(R_{a})^{2}+(X_{d}''\times X_{q}'')}
\end{equation*}
{\bfseries
States}

 $I_{d}$ \ \ Direct axis current \ 

 $I_{q}$ \ \ Quadrature axis current

 $E_{d}''$ \ \ Direct axis voltage behind transient reactance

 $E_{q}'$ \ \ Quadrature axis voltage behind transient reactance

 $E_{q}''$ \ \ Quadrature axis voltage behind sub-transient reactance

{\bfseries
Variables}

 $V_{d}$ \ \ Direct access component of terminal voltage

 $V_{q}$ \ \ Quadrature axis component of terminal voltage

 $V_{f}$ \ \ Field voltage referred to stator terminals

{\bfseries
Parameters}

 $T_{\mathit{qo}}''$ \ \ Quadrature axis open-circuit sub-transient time
constant

 $T_{\mathit{do}}'$ \ \ Direct axis open-circuit transient time constant

 $T_{\mathit{do}}''$ \ \ Direct axis open-circuit sub-transient time
constant

 $X_{d}$ \ \ Direct axis reactance

 $X_{d}'$ \ \ Direct axis transient reactance

 $X_{d}''$ \ \ Direct axis sub-transient reactance

 $X_{q}$ \ \ Quadrature axis reactance

 $X_{q}''$ \ \ Quadrature axis sub-transient reactance

 $R_{a}$ \ \ Winding resistance


\bigskip

 $\dot{x}_{n}$ \ \ The dot n\textsuperscript{th} state

 $x_{n}$ \ \ The n\textsuperscript{th} state

 $u_{n}$ \ \ The n\textsuperscript{th} input


$\left\{\begin{matrix}\dot{x}_{1}\\\dot{x}_{2}\\\dot{x}_{3}\\\dot{x}_{4}\\\dot{x}_{5}\end{matrix}\right\}=\left\{\begin{matrix}0&0&m_{1}&0&m_{2}\\0&0&m_{3}&0&m_{4}\\0&m_{5}&m_{6}&0&0\\m_{7}&0&0&m_{8}&0\\m_{9}&0&0&m_{10}&m_{11}\end{matrix}\right\}\left\{\begin{matrix}x_{1}\\x_{2}\\x_{3}\\x_{4}\\x_{5}\end{matrix}\right\}+\left\{\begin{matrix}n_{1}&n_{2}&0\\n_{3}&n_{4}&0\\0&0&0\\0&0&n_{5}\\0&0&0\end{matrix}\right\}\left\{\begin{matrix}u_{1}\\u_{2}\\u_{3}\end{matrix}\right\}$
$\begin{gathered}m_{1}=Y_{\Re
}\\m_{2}=-Y_{d}''\\m_{3}=-Y_{q}''\\m_{4}=Y_{\Re
}\\m_{5}=\frac{X_{q}-X_{q}''}{T_{\mathit{qo}}''}\\m_{6}=\frac{a-1}{T_{\mathit{qo}}''}\\m_{7}=\frac{X_{d}-X_{d}'}{T_{\mathit{do}}'}\\m_{8}=\frac{a-1}{T_{\mathit{do}}'}\\m_{9}=\frac{X_{d}'-X_{d}''}{T_{\mathit{do}}''}\\m_{10}=\frac{a+1}{T_{\mathit{do}}''}\\m_{11}=\frac{a-1}{T_{\mathit{do}}''}\end{gathered}$
$\begin{gathered}n_{1}=-Y_{\Re
}\\n_{2}=Y_{d}''\\n_{3}=Y_{q}''\\n_{4}=-Y_{\Re
}\\n_{5}=\frac{1}{T_{\mathit{do}}'}\end{gathered}$

Network Interface


\bigskip


\bigskip

\begin{equation*}
(E_{\Re }''+jE_{\Im }'')-(V_{\Re }+jV_{\Im })=(R_{a}+jX'').(I_{\Re
}+jI_{\Im })
\end{equation*}
or if there is a generator transformer:

\begin{equation*}
n\times (E_{\Re }''+jE_{\Im }'')-(V_{\Re }+jV_{\Im
})=(R_{a}+jX''+R_{t}+jX_{t})\times n\times (I_{\Re }+jI_{\Im })
\end{equation*}

\bigskip

\clearpage
States:\ \  $E_{d}',E_{d}'',E_{q}',E_{q}'',\omega ,\delta ,V_{a}$

Inputs:\ \ 
$aE_{d}',aE_{d}'',aE_{q}',aE_{q}'',T_{a},V_{d},V_{q},E_{\mathit{fd}}$(A.K.A.
non-integrable states)

Parameters:\ \ 
$\begin{gathered}x_{d},x_{d}',x_{d}'',x_{q},x_{q}',x_{q}'',T_{\mathit{do}}',T_{\mathit{do}}'',T_{\mathit{qo}}',T_{\mathit{qo}}''\\M,Y_{\Re
},Y_{\Im
},\mathit{Tap},D_{a},T_{\mathit{lo}},T_{\mathit{mo}},f_{\mathit{wm}},f_{0}=50\end{gathered}$(A.K.A.
constants)

States - PSSENG tsmmat.c 762 FormMachineMatrix(), 

\begin{equation*}
\begin{gathered}\dot{E}_{d}'=\frac{1}{T_{\mathit{qo}'}}\{-E_{d}'-aE_{d}'+I_{q}(x_{q}-x_{q}')\}\\\dot{E}_{d}''=\frac{1}{T_{\mathit{qo}''}}\{E_{d}'-E_{d}''+aE_{d}'-aE_{d}''+I_{q}(x_{q}'-x_{q}'')\}\\\dot{E}_{q}'=\frac{1}{T_{\mathit{do}'}}\{V_{a}-E_{q}'-aE_{q}'+I_{d}(x_{d}-x_{d}')\}\\\dot{E}_{q}''=\frac{1}{T_{\mathit{do}''}}\{E_{q}'-E_{q}''+aE_{q}'-aE_{q}''+I_{d}(x_{d}'-x_{d}'')\}\\\dot{\omega
}=T_{a}\div M\\\dot{\delta }=\omega \\\dot{V}_{a}=?\end{gathered}
\end{equation*}
Inputs (A.K.A. non-integrable states) - PSSENG tsmgrp.c 722
SolveMachineGroups()

\begin{equation*}
\begin{gathered}aE_{d}'=\alpha \cdot {E_{d}'}\cdot
{\frac{x_{q}}{x_{d}}}\\aE_{d}''=\alpha \cdot {E_{d}''}\cdot
{\frac{x_{q}}{x_{d}}}-(I_{q}\cdot (x_{q}-x_{q}')-E_{d}'-aE_{d}')\cdot
{\frac{T_{\mathit{qo}}''}{T_{\mathit{qo}}'}}\\aE_{q}'=\alpha \cdot
{E_{q}'}\\aE_{q}''=\alpha \cdot {E_{q}''}-(E_{\mathit{fd}}-I_{d}\cdot
(x_{d}-x_{d}')-E_{q}'-aE_{q}')\cdot
{\frac{T_{\mathit{do}}''}{T_{\mathit{do}}'}}\\T_{a}=t_{m}-t_{e}-T_{\mathit{lo}}-D_{a}\ast
\omega \\V_{d}=\frac{\sin (\delta )\cdot V_{\Re }+\cos (\delta )\cdot
V_{\Im }}{\mathit{Tap}}\\V_{q}=\frac{\cos (\delta )\cdot V_{\Re }+\sin
(\delta )\cdot V_{\Im
}}{\mathit{Tap}}\\E_{\mathit{fd}}=V_{a}\end{gathered}
\end{equation*}
Outputs:

 $\begin{gathered}I_{\Re }=\cos (\delta )\cdot I_{\mathit{njq}}+\sin
(\delta )\cdot I_{\mathit{njd}}\\I_{\Im }=\sin (\delta )\cdot
I_{\mathit{njq}}-\cos (\delta )\cdot I_{\mathit{njd}}\end{gathered}$
$\begin{gathered}I_{\mathit{njq}}=(Y_{g\Re }\cdot E_{q}'')+(Y_{g\Im
}\cdot E_{d}'')\\I_{\mathit{njd}}=(Y_{g\Re }\cdot E_{d}'')-(Y_{g\Im
}\cdot E_{q}'')\end{gathered}$

Where:

\begin{flushleft}
\tablefirsthead{}
\tablehead{}
\tabletail{}
\tablelasttail{}
\begin{supertabular}{|m{4.794cm}|m{7.896cm}|m{4.2980003cm}|}
\hline
\begin{equation*}
\begin{gathered}t_{m}=\frac{T_{\mathit{mo}}}{1.0+(\frac{\omega }{2\pi
\cdot f_{0}})}\\{}\\t_{e}=\frac{(E_{q}''\cdot {I_{q}})+(E_{d}''\cdot
{I_{d}})}{1.0+\frac{f_{\mathit{wm}}}{2\pi \cdot f_{0}}}\end{gathered}
\end{equation*}
 &
\begin{equation*}
\alpha
=\mathit{CalcSat}(\sqrt{(E_{q}'')^{2}+(E_{d}'')^{2}},\mathit{SatTab})
\end{equation*}
~

\begin{equation*}
\begin{gathered}I_{d}=Y_{\Re }(E_{d}''-V_{d})-Y_{\Im
}(E_{q}''-V_{q})\\I_{q}=Y_{\Re }(E_{q}''-V_{q})+Y_{\Im
}(E_{d}''-V_{d})\end{gathered}
\end{equation*}
~

 $(V_{\Re },V_{\Im })$ Bus Bar Voltages &
 $E_{\mathit{fd}},V_{a}$ Strange or only partly used states. 
$E_{\mathit{fd}}$ does not connect to a state. $V_{a}$ cannot change as
it doesn't have any elements in it's matrix row. \\\hline
\end{supertabular}
\end{flushleft}

\bigskip

\begin{equation*}
\begin{gathered}(I_{d}+j\cdot I_{q})\cdot (R_{a}+j\cdot
X'')=(E_{d}''+j\cdot E_{q}'')-(V_{d}-j\cdot V_{q})\\...\\I_{d}=Y_{\Re
}(E_{d}''-V_{d})-Y_{\Im }(E_{q}''-V_{q})\\I_{q}=Y_{\Re
}(E_{q}''-V_{q})+Y_{\Im }(E_{d}''-V_{d})\\I_{\Re }=\cos (\delta )\cdot
I_{q}+\sin (\delta )\cdot I_{d}\\I_{\Im }=\sin (\delta )\cdot
I_{q}-\cos (\delta )\cdot I_{d}\end{gathered}
\end{equation*}

\bigskip
\end{document}
